# Matrix Formulation

    Mn(w) = w^(jk)

    (n * n) matrix * (1 * n) vector

    | 1  1   1   1  ...     1     |   |  v1 |
    | 1  w  w^2 w^4 ...  w^(n-1)  |   |  v2 |
    | 1 w^2 w^4 w^8 ...  w^2(n^1) | x | ... |
    | ...  ...   ...  ...  ...    |   | ... |
    | 1 w^(n-1)  ... w^(n-1)(n-1) |   |  vn |

    = sum[0..(n-1)] of (w^(jk) * vj), k = 0 ... n-1
    = sum[even j] of (w^(jk) * vj) + sum[odd j] of (w^(jk) * vj)

    =   sum[0..(n/2 - 1)] of (w^2jk * v(2i))
      + wk * sum[0..(n/2 - 1)] of (w^2i * v(2i + 1))

# Hadamont Matrix

    H(m) = | H(m-1) | H(m-1) | x | y1 |
           | H(m-1) | H(m-1) |   | y2 |

    H(m-1) = | H(m-2) | H(m-2) | x | y1 |
             | H(m-2) | H(m-2) |   | y2 |

    = H(m-1)*y1 +- H(m-1)*y2

    =   (H(m-2) * y1,1 +- H(m-2) * y1,2)
      + (H(m-2) * y1,1 +- H(m-2) * y1,2)

What is the recurrence function of this?

    a = 2
    b = n/2

    T(n) = 2T(n/2) + O(N)

By the master theorm, that gives us a running time of:

    O(n^d * logb(n))
    O(n * log(n))

# Comparing Big-O Run Time

Compare `f(x) = log(n)^log(n)` and `g(x) = n^(log(log(n)))`

f(x):

    = 2^log(log(n)^log(n)) // raising to the 2 and logging are opposites
    = 2^(log(n) * log(log(n))) // Exponents in logs can come outside

g(x):

    = 2^log(n^(log(n)*log(n)))
    = 2^(log(log(n)) * log(n))

The running time is equal!


    log(n!) = Θ(n*log(n))
            = log(n) + log(n-1) + ... + log(2) + log(1)
            = SUM[1..N] of log(i)
            = ς log(i)di = [i * (log(i) - 1)]
            = n(log(n) - 1) + 1
            = n * log(n) - n + 1

